IsSupportedKeyManagerStrategy

AwsCryptographicMaterialProviders/dafny/AwsCryptographyKeyStoreAdmin/src/KmsUtils.dfy
@@ -1,6 +1,7 @@
 // Copyright Amazon.com Inc. or its affiliates. All Rights Reserved.
 // SPDX-License-Identifier: Apache-2.0
 include "../Model/AwsCryptographyKeyStoreAdminTypes.dfy"
+include "MutationStateStructures.dfy"
 
 module {:options "/functionSyntax:4" } KmsUtils {
   import opened Wrappers
@@ -8,6 +9,7 @@ module {:options "/functionSyntax:4" } KmsUtils {
   import KMSKeystoreOperations
   import KeyStoreTypes = KMSKeystoreOperations.Types
   import Types = AwsCryptographyKeyStoreAdminTypes
+  import StateStrucs = MutationStateStructures
   import KmsArn
 
   datatype KMSTuple = | KMSTuple(
@@ -137,5 +139,15 @@ module {:options "/functionSyntax:4" } KmsUtils {
     match kmsSymmetricArn
     case KmsKeyArn(kmsKeyArn) => KeyStoreTypes.kmsKeyArn(kmsKeyArn)
   }
+
+  predicate IsSupportedKeyManagerStrategy(
+    mutationToApply: StateStrucs.MutationToApply,
+    keyManagerStrategy: keyManagerStrat
+  )
+  {
+    && (mutationToApply.Terminal.hierarchyVersion.v1? ==> keyManagerStrategy.SupportHV1())
+    && (mutationToApply.Terminal.hierarchyVersion.v2? ==> keyManagerStrategy.SupportHV2())
+  }
+
 
 }
